Core/Interaction.v
@@ -1,0 +1,82 @@
+From Core Require Import
+  Specification
+  Signature
+  Program.
+
+From Util Require Import
+  Relation
+  Map.
+
+Definition AgentState (E F : Sig) :=
+  option ({R & prod (F R) (sum (Prog E R) {A & prod (E A) (A -> Prog E R)})}).
+Notation Idle :=
+  ( None
+  : AgentState _ _ ).
+Notation Cont m e :=
+  ( Some (existT _ _ (m, inl e))
+  : AgentState _ _ ).
+Notation Call om um k :=
+  ( Some (existT _ _ (om, inr (existT _ _ (um, k))))
+  : AgentState _ _ ).
+
+Definition AgentsState (T : nat) (E F : Sig) :=
+  Map (Agent T) (AgentState E F).
+
+Variant OSeqAgentStep {E F} {M : Mod E F} : Rel (SeqEvent F) (AgentState E F) :=
+| OInvStep R (om : F R) :
+  OSeqAgentStep Idle (InvEv om) (Cont om (M _ om))
+| ORetStep R (om : F R) v :
+  OSeqAgentStep (Cont om (Ret v)) (RetEv om v) Idle.
+Arguments OSeqAgentStep {E F} M.
+
+Variant USeqAgentStep {E F} : Rel (option (SeqEvent E)) (AgentState E F) :=
+| UInvStep R (om : F R) A (um : E A) k :
+  USeqAgentStep (Cont om (Vis um k)) (Some (InvEv um)) (Call om um k)
+| URetStep R (om : F R) A (um : E A) k v :
+  USeqAgentStep (Call om um k) (Some (RetEv um v)) (Cont om (k v))
+| UTauStep R (om : F R) e :
+  USeqAgentStep (Cont om (Tau e)) None (Cont om e).
+
+Definition InterState T E F A :=
+  prod (AgentsState T E F) A.
+
+Definition LEvent T E F :=
+  prod (Agent T) (sum (option (SeqEvent E)) (SeqEvent F)).
+
+Definition UEvent T E :=
+  prod (Agent T) (option (SeqEvent E)).
+
+Definition AgentStep {T E F} (M : Mod E F)
+: Rel (LEvent T E F) (AgentsState T E F) :=
+  PtRel (DisjRel USeqAgentStep (OSeqAgentStep M)).
+
+Definition ConcreteStep {T E F} (VE : Spec T E)
+: Rel (LEvent T E F) VE.(State) :=
+  fun s '(i, e) t =>
+    match e with
+    | inl (Some e) => VE.(Step) s (i, e) t
+    | _ => s = t
+    end.
+  
+Definition UnderConcreteStep {T E} (VE : Spec T E)
+: Rel (UEvent T E) VE.(State) :=
+  fun s '(i, e) t =>
+    match e with
+    | Some e => VE.(Step) s (i, e) t
+    | _ => s = t
+    end.
+
+Definition UnderInterStep {T E F}
+  (VE : Spec T E)
+: Rel (UEvent T E) (InterState T E F VE.(State)) :=
+  ConjRel (PtRel USeqAgentStep) (UnderConcreteStep VE).
+
+Definition InterStep {T E F}
+  (VE : Spec T E) (M : Mod E F)
+: Rel (LEvent T E F) (InterState T E F VE.(State)) :=
+  ConjRel (AgentStep M) (ConcreteStep VE).
+
+Definition InterSteps {T E F}
+  (VE : Spec T E) (M : Mod E F)
+: Rel (list (LEvent T E F)) (InterState T E F VE.(State)) :=
+  Steps (InterStep VE M).
