Core/Specification.v
@@ -1,0 +1,20 @@
+From Core Require Import
+  Signature.
+
+Definition Agent T := {i | i < T}.
+
+Definition SeqEvent (E : Sig) :=
+  {A & prod (E A) (option A)}.
+
+Notation Evt m r := (existT _ _ (m, r)).
+Notation InvEv m := (Evt m None).
+Notation RetEv m v := (Evt m (Some v)).
+
+Definition Event T E : Type := Agent T * SeqEvent E.
+
+Record Spec {T E} : Type := {
+  State : Type;
+  Init : State;
+  Step : State -> Event T E -> State -> Prop;
+}.
+Arguments Spec : clear implicits.
