Util/Relation.v
@@ -1,0 +1,29 @@
+From Util Require Import
+  Map.
+
+Definition Rel E A := A -> E -> A -> Prop.
+
+Variant PtRel {E I A} {R : Rel E A} : Rel (I * E) (Map I A) :=
+| MkPtRel m i e x y : R x e y -> PtRel (m [i ↦ x]) (i, e) (m [i ↦ y]).
+Arguments PtRel {E I A} R.
+
+Variant ConjRel {E A B} {RL : Rel E A} {RR : Rel E B} : Rel E (prod A B) :=
+| MkConjRel e x z y w :
+  RL x e z ->
+  RR y e w ->
+  ConjRel (x, y) e (z, w).
+Arguments ConjRel {E A B} RL RR.
+
+Variant DisjRel {E F A} {RL : Rel E A} {RR : Rel F A} : Rel (sum E F) A :=
+| DisjRelLeft e x y :
+  RL x e y ->
+  DisjRel x (inl e) y
+| DisjRelRight e x y :
+  RR x e y ->
+  DisjRel x (inr e) y.
+Arguments DisjRel {E F A} RL RR.
+
+Inductive Steps {E A} {R : Rel E A} : Rel (list E) A :=
+| StepsNil x : Steps x nil x
+| StepsCons e p x y z : R x e y -> Steps y p z -> Steps x (cons e p) z.
+Arguments Steps {E A} R.
